Add zip, unzip, filer.

src/dafny/utils/MiscTypes.dfy
@@ -43,4 +43,30 @@ module MiscTypes {
     }
   }
 
+  function Zip<U, V>(u: seq<U>, v: seq<V>): seq<(U, V)>
+    requires |u| == |v|
+  {
+    seq(|u|, i requires 0 <= i < |u| => (u[i], v[i]))
+  }
+
+  function UnZip<U, V>(x: seq<(U, V)>): (seq<U>, seq<V>)
+    ensures |UnZip(x).0| == |UnZip(x).1| == |x|
+    ensures forall k:: 0 <= k < |x| ==> (UnZip(x).0[k] == x[k].0 && UnZip(x).1[k] == x[k].1)
+  {
+    var x0 := seq(|x|, i requires 0 <= i < |x| => x[i].0);
+    var x1 := seq(|x|, i requires 0 <= i < |x| => x[i].1);
+    (x0 ,x1)
+  }
+
+  function Filter<U>(u: seq<U>, f: U -> bool): (r: seq<U>)
+    ensures |r| <= |u|
+    ensures forall x:: x in r ==> x in u
+    ensures forall k:: 0 <= k < |r| ==> f(r[k]) 
+    ensures forall x:: x in r ==> f(x)
+  {
+    if |u| == 0 then [] 
+    else if f(u[0]) then [u[0]] + Filter(u[1..], f)
+    else Filter(u[1..], f)
+  }
+
 }
